sort out universe level handling

tests/lean/run/derivingToExpr.lean
@@ -1,69 +1,140 @@
 import Lean.Elab.Deriving.ToExpr
 
+/-!
+# Tests for the `ToExpr` deriving handler
+-/
+
 open Lean
 
-deriving instance ToExpr for ULift
-
--- Test with empty type
-inductive Empty'
-  deriving ToExpr
-
--- Test without universes
+/-!
+Test without universes
+-/
 inductive MonoOption' (α : Type) : Type
   | some (a : α)
   | none
   deriving ToExpr
 
--- Test with a universe polymporphic type parameter
+/--
+info: Lean.Expr.app
+  (Lean.Expr.app (Lean.Expr.const `MonoOption'.some []) (Lean.Expr.const `Bool []))
+  (Lean.Expr.const `Bool.true [])
+-/
+#guard_msgs in
+#eval repr <| toExpr <| MonoOption'.some true
+
+/-!
+Test with a universe polymorphic type parameter
+-/
 inductive Option' (α : Type u)
   | some (a : α)
   | none
   deriving ToExpr
 
-/-- info: instToExprOption'OfToLevel -/
-#guard_msgs in #synth ToExpr (Option' Nat)
-/-- info: instToExprOption'OfToLevel -/
-#guard_msgs in #synth ToExpr (Option' <| ULift.{20} Nat)
+/--
+info: Lean.Expr.app
+  (Lean.Expr.app (Lean.Expr.const `Option'.some [Lean.Level.zero]) (Lean.Expr.const `Bool []))
+  (Lean.Expr.const `Bool.true [])
+-/
+#guard_msgs in
+#eval repr <| toExpr <| Option'.some true
+
+example : ToExpr (Option' Nat) := inferInstance
+
+/-!
+Test with higher universe levels
+-/
+structure MyULift.{r, s} (α : Type s) : Type (max s r) where
+  up :: down : α
+  deriving ToExpr
 
 /--
 info: Lean.Expr.app
   (Lean.Expr.app
-    (Lean.Expr.const `Option'.some [Lean.Level.succ (Lean.Level.succ (Lean.Level.succ (Lean.Level.zero)))])
+    (Lean.Expr.const `Option'.some [Lean.Level.succ (Lean.Level.succ (Lean.Level.zero))])
     (Lean.Expr.app
-      (Lean.Expr.const `ULift [Lean.Level.succ (Lean.Level.succ (Lean.Level.succ (Lean.Level.zero))), Lean.Level.zero])
-      (Lean.Expr.const `Nat [])))
+      (Lean.Expr.const `MyULift [Lean.Level.succ (Lean.Level.succ (Lean.Level.zero)), Lean.Level.zero])
+      (Lean.Expr.const `Bool [])))
   (Lean.Expr.app
     (Lean.Expr.app
-      (Lean.Expr.const
-        `ULift.up
-        [Lean.Level.succ (Lean.Level.succ (Lean.Level.succ (Lean.Level.zero))), Lean.Level.zero])
-      (Lean.Expr.const `Nat []))
-    (Lean.Expr.app
-      (Lean.Expr.app
-        (Lean.Expr.app (Lean.Expr.const `OfNat.ofNat [Lean.Level.zero]) (Lean.Expr.const `Nat []))
-        (Lean.Expr.lit (Lean.Literal.natVal 42)))
-      (Lean.Expr.app (Lean.Expr.const `instOfNatNat []) (Lean.Expr.lit (Lean.Literal.natVal 42)))))
+      (Lean.Expr.const `MyULift.up [Lean.Level.succ (Lean.Level.succ (Lean.Level.zero)), Lean.Level.zero])
+      (Lean.Expr.const `Bool []))
+    (Lean.Expr.const `Bool.true []))
 -/
-#guard_msgs in #eval toExpr (Option'.some <| ULift.up.{3} 42)
+#guard_msgs in
+#eval repr <| toExpr <| Option'.some (MyULift.up.{2} true)
 
--- Test with recursive type
+example : ToExpr (Option' <| MyULift.{20} Nat) := inferInstance
+example [ToLevel.{u}] : ToExpr (Option' <| MyULift.{u} Nat) := inferInstance
+
+/-!
+Test with empty type.
+-/
+inductive Empty'
+  deriving ToExpr
+
+/-!
+Test with recursive type
+-/
 inductive List' (α : Type u)
   | cons (a : α) (as : List' α)
   | nil
   deriving ToExpr
 
+/-!
+Test with nested type
+-/
+inductive Foo
+  | l (x : List Foo)
+  deriving ToExpr
+
+/-!
+Test with mutual inductive type
+-/
+mutual
+inductive A
+  | nil
+  | cons (a : A) (b : B)
+  deriving ToExpr
+inductive B
+  | cons₁ (a : A)
+  | cons₂ (a : A) (b : B)
+  deriving ToExpr
+end
+
+/--
+info: Lean.Expr.app
+  (Lean.Expr.app (Lean.Expr.const `A.cons []) (Lean.Expr.const `A.nil []))
+  (Lean.Expr.app (Lean.Expr.const `B.cons₁ []) (Lean.Expr.const `A.nil []))
+-/
+#guard_msgs in
+#eval repr <| toExpr <| A.cons A.nil (B.cons₁ A.nil)
+/--
+info: Lean.Expr.app
+  (Lean.Expr.app (Lean.Expr.const `B.cons₂ []) (Lean.Expr.const `A.nil []))
+  (Lean.Expr.app (Lean.Expr.const `B.cons₁ []) (Lean.Expr.const `A.nil []))
+-/
+#guard_msgs in
+#eval repr <| toExpr <| B.cons₂ A.nil (B.cons₁ A.nil)
+
+/-!
+Test with explicit universe level
+-/
+
 inductive WithUniverse.{u} (α : Type u)
   | foo (a : α)
   deriving ToExpr
 
+/-!
+Test with universe level coming from `universe` command
+-/
 universe u in
 inductive WithAmbientUniverse (α : Type u)
   | foo (a : α)
   deriving ToExpr
 
-set_option trace.Elab.Deriving.toExpr true in
--- A test with: an ambient universe `u`, a directly specified universe `v`, and
--- an implicit universe `w`
+/-!
+Test with an ambient universe `u`, a directly specified universe `v`, and an implicit universe `w`.
+-/
 universe u in
 structure WithAmbientUniverseTriple.{v} (α : Type u) (β : Type v) (γ : Type w) where
   a : α
@@ -71,24 +142,59 @@ structure WithAmbientUniverseTriple.{v} (α : Type u) (β : Type v) (γ : Type w
   c : γ
   deriving ToExpr
 
--- Tests without (universe) auto implicits
+/-!
+Test using the `variable` command, with an autoimplicit universe.
+-/
+variable (α : Type u) in
+inductive VariableParameter : Type u
+  | foo (a : α)
+  deriving ToExpr
+
+/-!
+Mutual inductive with universe levels.
+-/
+mutual
+inductive A' (α : Type u) where
+  | mk (x : α) (a : A' α) (b : B' α)
+  deriving ToExpr
+inductive B' (α : Type u) where
+  | mk (x : α) (a : A' α) (b : B' α)
+  deriving ToExpr
+end
+
+/-!
+Nested with universe level.
+-/
+inductive Foo' (α : Type u)
+  | l (x : α) (x : List (Foo' α))
+  deriving ToExpr
+
+/-!
+### Tests with without universe autoimplicits.
+-/
 section NoAutoImplicit
 set_option autoImplicit false
 
--- Test with universe specified directly on the type
+/-!
+Test with universe specified directly on the type
+-/
 inductive ExplicitList'.{u} (α : Type u)
   | cons (a : α) (as : List' α)
   | nil
   deriving ToExpr
 
--- Test with ambient (explicit) universe
+/-!
+Test with ambient (explicit) universe
+-/
 universe u in
 inductive AmbientList' (α : Type u)
   | cons (a : α) (as : List' α)
   | nil
   deriving ToExpr
 
--- Now, test both ambient and directly specified universes
+/-!
+Test with both ambient and directly specified universes.
+-/
 universe u in
 structure ExplicitAmbientPair.{v} (α : Type u) (β : Type v) where
   a : α
@@ -96,14 +202,3 @@ structure ExplicitAmbientPair.{v} (α : Type u) (β : Type v) where
   deriving ToExpr
 
 end NoAutoImplicit
-
--- Test with an implicit parameter to the inductive type
-inductive ImplicitParameter
-  | foo (a : α)
-  deriving ToExpr
-
--- Test where the type parameter is a variable, with an implicit universe
-variable {α : Type u} in
-inductive VariableParameter : Type
-  | foo (a : α)
-  deriving ToExpr
