src/Lean/Elab/Deriving/ToExpr.lean
@@ -1,5 +1,5 @@
 /-
-Copyright (c) 2023 Kyle Miller. All rights reserved.
+Copyright (c) 2024 Lean FRO, LLC. All rights reserved.
 Released under Apache 2.0 license as described in the file LICENSE.
 Authors: Kyle Miller
 -/
@@ -7,46 +7,67 @@ prelude
 import Lean.Meta.Transform
 import Lean.Elab.Deriving.Basic
 import Lean.Elab.Deriving.Util
-import Lean.ToExpr
 import Lean.ToLevel
-
+import Lean.ToExpr
 
 /-!
-# A `ToExpr` derive handler
+# `ToExpr` deriving handler
 
-This module defines a `ToExpr` derive handler for inductive types. It supports mutually inductive
-types as well.
+This module defines a `ToExpr` deriving handler for inductive types.
+It supports mutually inductive types as well.
 
-The `ToExpr` derive handlers support universe level polymorphism. This is implemented using the
-`Lean.ToLevel` class. To use `ToExpr` in places where there is universe polymorphism, make sure
-to have a `[ToLevel.{u}]` instance available.
+The `ToExpr` deriving handlers support universe level polymorphism, via the `Lean.ToLevel` class.
+To use `ToExpr` in places where there is universe polymorphism, make sure a `[ToLevel.{u}]` instance is available,
+though be aware that the `ToLevel` mechanism does not support `max` or `imax` expressions.
 
-Implementation note: this derive handler was originally modeled after the `Repr` derive handler.
+Implementation note: this deriving handler was initially modeled after the `Repr` deriving handler, but
+1. we need to account for universe levels,
+2. the `ToExpr` class has two fields rather than one, and
+3. we don't handle structures specially.
 -/
 
 namespace Lean.Elab.Deriving.ToExpr
 
-open Lean Elab Lean.Parser.Term
+open Lean Elab Parser.Term
 open Meta Command Deriving
 
-/-- Specialization of `Lean.Elab.Deriving.mkHeader` for `ToExpr`. -/
-def mkToExprHeader (indVal : InductiveVal) : TermElabM Header := do
-  -- The auxiliary functions we produce are `indtype -> Expr`.
-  let header ← mkHeader ``ToExpr 1 indVal
-  return header
-
-/-- Give a term that is equivalent to `(term| mkAppN $f #[$args,*])`.
-As an optimization, `mkAppN` is pre-expanded out to use `Expr.app` directly. -/
+/--
+Given `args := #[e₁, e₂, …, eₙ]`, constructs the syntax `Expr.app (… (Expr.app (Expr.app f e₁) e₂) …) eₙ`.
+-/
 def mkAppNTerm (f : Term) (args : Array Term) : MetaM Term :=
-  args.foldlM (fun a b => `(Expr.app $a $b)) f
+  args.foldlM (fun a b => ``(Expr.app $a $b)) f
 
-/-- Create the body of the `toExpr` function
-for the `ToExpr` instance, which is a `match` expression
+/-- Fixes the output of `mkInductiveApp` to explicitly reference universe levels. -/
+def updateIndType (indVal : InductiveVal) (t : Term) : TermElabM Term :=
+  match t with
+  | `(@$f $args*) =>
+    let levels := indVal.levelParams.toArray.map mkIdent
+    `(@$f.{$levels,*} $args*)
+  | _ => throwError "(internal error) expecting output of `mkInductiveApp`"
+
+/--
+Creates a term that evaluates to an expression representing the inductive type.
+Uses `toExpr` and `toTypeExpr` for the arguments to the type constructor.
+-/
+def mkToTypeExpr (indVal : InductiveVal) (argNames : Array Name) : TermElabM Term := do
+  let levels ← indVal.levelParams.toArray.mapM (fun u => `(Lean.toLevel.{$(mkIdent u)}))
+  forallTelescopeReducing indVal.type fun xs _ => do
+    let mut args : Array Term := #[]
+    for argName in argNames, x in xs do
+      let a := mkIdent argName
+      if ← Meta.isType x then
+        args := args.push <| ← ``(toTypeExpr $a)
+      else
+        args := args.push <| ← ``(toExpr $a)
+    mkAppNTerm (← ``((Expr.const $(quote indVal.name) [$levels,*]))) args
+
+/--
+Creates the body of the `toExpr` function for the `ToExpr` instance, which is a `match` expression
 that calls `toExpr` and `toTypeExpr` to assemble an expression for a given term.
-For recursive inductive types, `auxFunName` refers to the `ToExpr` instance
-for the current type.
-For mutually recursive types, we rely on the local instances set up by `mkLocalInstanceLetDecls`. -/
-def mkToExprBody (header : Header) (indVal : InductiveVal) (auxFunName : Name) :
+For recursive inductive types, `auxFunName` refers to the `ToExpr` instance for the current type.
+For mutually recursive types, we rely on the local instances set up by `mkLocalInstanceLetDecls`.
+-/
+def mkToExprBody (header : Header) (indVal : InductiveVal) (auxFunName : Name) (levelInsts : Array Term) :
     TermElabM Term := do
   let discrs ← mkDiscrs header indVal
   let alts ← mkAlts
@@ -54,23 +75,24 @@ def mkToExprBody (header : Header) (indVal : InductiveVal) (auxFunName : Name) :
 where
   /-- Create the `match` cases, one per constructor. -/
   mkAlts : TermElabM (Array (TSyntax ``matchAlt)) := do
+    let levels ← levelInsts.mapM fun inst => `($(inst).toLevel)
     let mut alts := #[]
     for ctorName in indVal.ctors do
       let ctorInfo ← getConstInfoCtor ctorName
       let alt ← forallTelescopeReducing ctorInfo.type fun xs _ => do
         let mut patterns := #[]
-        -- add `_` pattern for indices
+        -- add `_` pattern for indices, before the constructor's pattern
         for _ in [:indVal.numIndices] do
           patterns := patterns.push (← `(_))
         let mut ctorArgs := #[]
         let mut rhsArgs : Array Term := #[]
         let mkArg (x : Expr) (a : Term) : TermElabM Term := do
           if (← inferType x).isAppOf indVal.name then
-            `($(mkIdent auxFunName) $a)
+            `($(mkIdent auxFunName) $levelInsts* $a)
           else if ← Meta.isType x then
-            `(toTypeExpr $a)
+            ``(toTypeExpr $a)
           else
-            `(toExpr $a)
+            ``(toExpr $a)
         -- add `_` pattern for inductive parameters, which are inaccessible
         for i in [:ctorInfo.numParams] do
           let a := mkIdent header.argNames[i]!
@@ -81,39 +103,22 @@ where
           ctorArgs := ctorArgs.push a
           rhsArgs := rhsArgs.push <| ← mkArg xs[ctorInfo.numParams + i]! a
         patterns := patterns.push (← `(@$(mkIdent ctorName):ident $ctorArgs:term*))
-        let levels ← indVal.levelParams.toArray.mapM (fun u => `(toLevel.{$(mkIdent u)}))
-        let rhs : Term ←
-          mkAppNTerm (← `(Expr.const $(quote ctorInfo.name) [$levels,*])) rhsArgs
+        let rhs : Term ← mkAppNTerm (← ``(Expr.const $(quote ctorInfo.name) [$levels,*])) rhsArgs
         `(matchAltExpr| | $[$patterns:term],* => $rhs)
       alts := alts.push alt
     return alts
 
-/-- Create the body of the `toTypeExpr` function for the `ToExpr` instance.
-Calls `toExpr` and `toTypeExpr` to the arguments to the type constructor. -/
-def mkToTypeExpr (argNames : Array Name) (indVal : InductiveVal) : TermElabM Term := do
-  let levels ← indVal.levelParams.toArray.mapM (fun u => `(toLevel.{$(mkIdent u)}))
-  forallTelescopeReducing indVal.type fun xs _ => do
-    let mut args : Array Term := #[]
-    for i in [:xs.size] do
-      let x := xs[i]!
-      let a := mkIdent argNames[i]!
-      if ← Meta.isType x then
-        args := args.push <| ← `(toTypeExpr $a)
-      else
-        args := args.push <| ← `(toExpr $a)
-    mkAppNTerm (← `((Expr.const $(quote indVal.name) [$levels,*]))) args
-
 /--
-For mutually recursive inductive types, the strategy is to have local `ToExpr` instances in scope
-for each of the inductives when defining each instance.
-This way, each instance can freely use `toExpr` and `toTypeExpr` for each of the other types.
+For nested and mutually recursive inductive types, we define `partial` instances,
+and the strategy is to have local `ToExpr` instances in scope for the body of each instance.
+This way, each instance can freely use `toExpr` and `toTypeExpr` for each of the types in `ctx`.
 
-Note that each instance gets its own definition of each of the others' `toTypeExpr` fields.
-(This is working around the fact that the `Deriving.Context` API assumes
-that each instance in mutual recursion only has a single auxiliary definition.
-There are other ways to work around it, but `toTypeExpr` implementations
-are very simple, so duplicating them seemed to be OK.) -/
-def mkLocalInstanceLetDecls (ctx : Deriving.Context) (argNames : Array Name) :
+This is a modified copy of `Lean.Elab.Deriving.mkLocalInstanceLetDecls`,
+since we need to include the `toTypeExpr` field in the `letDecl`
+Note that, for simplicity, each instance gets its own definition of each others' `toTypeExpr` fields.
+These are very simple fields, so avoiding the duplication is not worth it.
+-/
+def mkLocalInstanceLetDecls (ctx : Deriving.Context) (argNames : Array Name) (levelInsts : Array Term) :
     TermElabM (Array (TSyntax ``Parser.Term.letDecl)) := do
   let mut letDecls := #[]
   for i in [:ctx.typeInfos.size] do
@@ -126,110 +131,98 @@ def mkLocalInstanceLetDecls (ctx : Deriving.Context) (argNames : Array Name) :
     let argNamesNew  := argNames[:numParams] ++ currIndices
     let indType      ← mkInductiveApp indVal argNamesNew
     let instName     ← mkFreshUserName `localinst
-    let toTypeExpr   ← mkToTypeExpr argNames indVal
-    let letDecl      ← `(Parser.Term.letDecl| $(mkIdent instName):ident $binders:implicitBinder* :
-                            ToExpr $indType :=
-                          { toExpr := $(mkIdent auxFunName), toTypeExpr := $toTypeExpr })
+    let toTypeExpr   ← mkToTypeExpr indVal argNames
+    -- Recall that each type uses the same universe levels.
+    let letDecl      ← `(Parser.Term.letDecl| $(mkIdent instName):ident $binders:implicitBinder* : ToExpr $indType :=
+                          { toExpr := $(mkIdent auxFunName) $levelInsts*, toTypeExpr := $toTypeExpr })
     letDecls := letDecls.push letDecl
   return letDecls
 
-/-- Fix the output of `mkInductiveApp` to explicitly reference universe levels. -/
-def fixIndType (indVal : InductiveVal) (t : Term) : TermElabM Term :=
-  match t with
-  | `(@$f $args*) =>
-    let levels := indVal.levelParams.toArray.map mkIdent
-    `(@$f.{$levels,*} $args*)
-  | _ => throwError "(internal error) expecting output of `mkInductiveApp`"
-
-/-- Make `ToLevel` instance binders for all the level variables. -/
-def mkToLevelBinders (indVal : InductiveVal) : TermElabM (TSyntaxArray ``instBinderF) := do
-  indVal.levelParams.toArray.mapM (fun u => `(instBinderF| [ToLevel.{$(mkIdent u)}]))
-
 open TSyntax.Compat in
-/-- Make a `toExpr` function for the given inductive type.
-The implementations of each `toExpr` function for a (mutual) inductive type
-are given as top-level private definitions.
-These end up being assembled into `ToExpr` instances in `mkInstanceCmds`.
-For mutual inductive types,
-then each of the other types' `ToExpr` instances are provided as local instances,
-to wire together the recursion (this necessitates these auxiliary definitions being `partial`). -/
+/--
+Makes a `toExpr` function for the given inductive type.
+The implementation of each `toExpr` function for a (mutual) inductive type is given as top-level private definitions.
+These are assembled into `ToExpr` instances in `mkInstanceCmds`.
+For mutual/nested inductive types, then each of the types' `ToExpr` instances are provided as local instances,
+to wire together the recursion (necessitating these auxiliary definitions being `partial`).
+-/
 def mkAuxFunction (ctx : Deriving.Context) (i : Nat) : TermElabM Command := do
   let auxFunName := ctx.auxFunNames[i]!
   let indVal     := ctx.typeInfos[i]!
-  let header     ← mkToExprHeader indVal
-  let mut body   ← mkToExprBody header indVal auxFunName
+  let header     ← mkHeader ``ToExpr 1 indVal
+  let (toLevelInsts, levelBinders) := Array.unzip <| ← indVal.levelParams.toArray.mapM fun u => do
+    let inst := mkIdent (← mkFreshUserName `inst)
+    return (inst, ← `(explicitBinderF| ($inst : ToLevel.{$(mkIdent u)})))
+  let mut body   ← mkToExprBody header indVal auxFunName toLevelInsts
   if ctx.usePartial then
-    let letDecls ← mkLocalInstanceLetDecls ctx header.argNames
+    let letDecls ← mkLocalInstanceLetDecls ctx header.argNames toLevelInsts
     body ← mkLet letDecls body
   -- We need to alter the last binder (the one for the "target") to have explicit universe levels
   -- so that the `ToLevel` instance arguments can use them.
   let addLevels binder :=
     match binder with
-    | `(bracketedBinderF| ($a : $ty)) => do `(bracketedBinderF| ($a : $(← fixIndType indVal ty)))
+    | `(bracketedBinderF| ($a : $ty)) => do `(bracketedBinderF| ($a : $(← updateIndType indVal ty)))
     | _ => throwError "(internal error) expecting inst binder"
-  let binders := header.binders.pop
-    ++ (← mkToLevelBinders indVal)
-    ++ #[← addLevels header.binders.back!]
-  let ambient ← Term.getLevelNames
-  let levels := indVal.levelParams.filter (· ∉ ambient) |>.toArray.map mkIdent
+  let binders := header.binders.pop ++ levelBinders ++ #[← addLevels header.binders.back!]
   if ctx.usePartial then
-    `(private partial def $(mkIdent auxFunName):ident.{$levels,*} $binders:bracketedBinder* :
-        Expr := $body:term)
+    `(private partial def $(mkIdent auxFunName):ident $binders:bracketedBinder* : Expr := $body:term)
   else
-    `(private def $(mkIdent auxFunName):ident.{$levels,*} $binders:bracketedBinder* :
-        Expr := $body:term)
+    `(private         def $(mkIdent auxFunName):ident $binders:bracketedBinder* : Expr := $body:term)
 
-/-- Create all the auxiliary functions using `mkAuxFunction` for the (mutual) inductive type(s).
-Wraps the resulting definition commands in `mutual ... end`. -/
-def mkMutualBlock (ctx : Deriving.Context) : TermElabM Syntax := do
+/--
+Creates all the auxiliary functions (using `mkAuxFunction`) for the (mutual) inductive type(s).
+Wraps the resulting definition commands in `mutual ... end`.
+-/
+def mkAuxFunctions (ctx : Deriving.Context) : TermElabM Syntax := do
   let mut auxDefs := #[]
   for i in [:ctx.typeInfos.size] do
     auxDefs := auxDefs.push (← mkAuxFunction ctx i)
   `(mutual $auxDefs:command* end)
 
 open TSyntax.Compat in
-/-- Assuming all of the auxiliary definitions exist, create all the `instance` commands
-for the `ToExpr` instances for the (mutual) inductive type(s). -/
+/--
+Assuming all of the auxiliary definitions exist,
+creates all the `instance` commands for the `ToExpr` instances for the (mutual) inductive type(s).
+This is a modified copy of `Lean.Elab.Deriving.mkInstanceCmds` to account for `ToLevel` instances.
+-/
 def mkInstanceCmds (ctx : Deriving.Context) (typeNames : Array Name) :
     TermElabM (Array Command) := do
   let mut instances := #[]
-  for i in [:ctx.typeInfos.size] do
-    let indVal       := ctx.typeInfos[i]!
+  for indVal in ctx.typeInfos, auxFunName in ctx.auxFunNames do
     if typeNames.contains indVal.name then
-      let auxFunName   := ctx.auxFunNames[i]!
       let argNames     ← mkInductArgNames indVal
       let binders      ← mkImplicitBinders argNames
       let binders      := binders ++ (← mkInstImplicitBinders ``ToExpr indVal argNames)
-      let binders      := binders ++ (← mkToLevelBinders indVal)
-      let indType      ← fixIndType indVal (← mkInductiveApp indVal argNames)
-      let toTypeExpr   ← mkToTypeExpr argNames indVal
-      let levels       := indVal.levelParams.toArray.map mkIdent
-      let ambientLevels ← Term.getLevelNames
-      /- `defLevels` are the universes which are *not* globally specified (via a `universe` command)
-          and need to be declared for the instance -/
-      let defLevels    := levels.filter (·.getId ∉ ambientLevels)
-      trace[Elab.Deriving.toExpr] "ambient levels: {← Term.getLevelNames}"
-      trace[Elab.Deriving.toExpr] "levels: {levels}"
-      trace[Elab.Deriving.toExpr] "defLevels: {defLevels}"
-      let instCmd ← `(universe $defLevels:ident* in
-                      instance $binders:implicitBinder* : ToExpr $indType where
-                        toExpr := $(mkIdent auxFunName).{$levels,*}
+      let (toLevelInsts, levelBinders) := Array.unzip <| ← indVal.levelParams.toArray.mapM fun u => do
+        let inst := mkIdent (← mkFreshUserName `inst)
+        return (inst, ← `(instBinderF| [$inst : ToLevel.{$(mkIdent u)}]))
+      let binders      := binders ++ levelBinders
+      let indType      ← updateIndType indVal (← mkInductiveApp indVal argNames)
+      let toTypeExpr   ← mkToTypeExpr indVal argNames
+      let instCmd ← `(instance $binders:implicitBinder* : ToExpr $indType where
+                        toExpr := $(mkIdent auxFunName) $toLevelInsts*
                         toTypeExpr := $toTypeExpr)
       instances := instances.push instCmd
   return instances
 
-/-- Returns all the commands generated by `mkMutualBlock` and `mkInstanceCmds`. -/
+/--
+Returns all the commands necessary to construct the `ToExpr` instances.
+-/
 def mkToExprInstanceCmds (declNames : Array Name) : TermElabM (Array Syntax) := do
   let ctx ← mkContext "toExpr" declNames[0]!
-  let cmds := #[← mkMutualBlock ctx] ++ (← mkInstanceCmds ctx declNames)
+  let cmds := #[← mkAuxFunctions ctx] ++ (← mkInstanceCmds ctx declNames)
   trace[Elab.Deriving.toExpr] "\n{cmds}"
   return cmds
 
-/-- The main entry point to the `ToExpr` derive handler. -/
+/--
+The main entry point to the `ToExpr` deriving handler.
+-/
 def mkToExprInstanceHandler (declNames : Array Name) : CommandElabM Bool := do
   if (← declNames.allM isInductive) && declNames.size > 0 then
-    let cmds ← liftTermElabM <| mkToExprInstanceCmds declNames
-    cmds.forM elabCommand
+    let cmds ← withFreshMacroScope <| liftTermElabM <| mkToExprInstanceCmds declNames
+    -- Enable autoimplicits for universe levels.
+    withScope (fun scope => { scope with opts := autoImplicit.set scope.opts true }) do
+      elabCommand (mkNullNode cmds)
     return true
   else
     return false
